proof/SystemF/Name.v
@@ -2,21 +2,60 @@
 
 Require Export Base.
 
-(* Names. We just use a nat for the unique id *)
-Inductive name : Type :=
- Name : nat -> name.
 
+(* Space *************************************************)
+Inductive space : Type :=
+ | SpaceValue 
+ | SpaceType.
+
+Definition beq_space s1 s2 :=
+ match (s1, s2) with
+  | (SpaceValue, SpaceValue) => true
+  | (SpaceType,  SpaceType)  => true
+  | (_, _)                   => false
+ end.
+
+Hint Unfold beq_space.
+
+
+Theorem beq_space_refl
+ : forall s
+ , true = beq_space s s.
+Proof.
+ intros.
+ destruct s; eauto.
+Qed.
+
+
+Theorem beq_space_sym
+ : forall s1 s2
+ , beq_space s1 s2 = beq_space s2 s1.
+Proof.
+ intros.
+ destruct s1. destruct s2; auto. auto.
+Qed.
+
+
+(* Names *************************************************)
+Inductive name : Type :=
+ Name : space -> nat -> name.
 
 (* Example names *)
-Notation nA := (Name 0).
-Notation nB := (Name 1).
-Notation nC := (Name 2).
+Notation xA := (Name SpaceValue 0).
+Notation xB := (Name SpaceValue 1).
+Notation xC := (Name SpaceValue 2).
 
 
 (* Names are equal when their ids are equal. *)
 Definition beq_name n1 n2 := 
  match (n1, n2) with 
-  (Name x1, Name x2) => beq_nat x1 x2
+  |  (Name SpaceValue x1, Name SpaceValue x2)
+  => beq_nat x1 x2
+
+  |  (Name SpaceType  x1, Name SpaceType  x2)
+  => beq_nat x1 x2
+
+  |  (_, _) => false
  end.
 
 Hint Unfold beq_name.
@@ -27,7 +66,8 @@ Theorem beq_name_refl
  : forall n
  , true = beq_name n n.
 Proof.
- intros. destruct n. unfold beq_name. apply beq_nat_refl.
+ intros. destruct n. destruct s;
+ unfold beq_name; apply beq_nat_refl.
 Qed.
 
 Hint Resolve beq_name_refl.
@@ -39,9 +79,13 @@ Theorem beq_name_sym
  , beq_name n1 n2 = beq_name n2 n1.
 Proof.
  intros.
- destruct n1. destruct n2.
- unfold beq_name.
- apply beq_nat_sym.
+ destruct n1. destruct n2. destruct s. destruct s0.
+ unfold beq_name. rewrite beq_nat_sym. auto.
+ unfold beq_name. trivial.
+ destruct s0.
+ unfold beq_name. trivial.
+ unfold beq_name. 
+ rewrite beq_nat_sym. trivial.
 Qed.
 
 
@@ -51,8 +95,24 @@ Theorem true_name_eq
 Proof.
  intros n1 n2. 
  destruct n1.  destruct n2.
+ destruct s.   destruct s0.
+  unfold beq_name. intro. apply true_nat_eq in H. subst. auto.
+  unfold beq_name. intro. inversion H.
+  destruct s0. 
+  unfold beq_name. intro. inversion H.
+  
+
+eapply beq_nat_refl in H.
+  intro.
  unfold beq_name. 
- intro. apply true_nat_eq in H. subst. trivial.
+ intro. destruct H.
+ eapply band_conj in H.
+ destruct s. destruct n0. 
+ unfold band in H. simpl.
+
+
+unfold band.
+ apply true_nat_eq in H. subst. trivial.
 Qed.
 
 Hint Resolve true_name_eq.
@@ -88,4 +148,7 @@ Proof.
  destruct n1. destruct n2.
  unfold beq_name. apply neq_nat_false. contradict H. subst. trivial.
 Qed.
+
+
+
 
