proof/SystemF/EvJudge.v
@@ -2,11 +2,11 @@
 Require Export Exp.
 
 Inductive STEP : exp -> exp -> Prop := 
-  | EVAppAbs 
+  | EVAppLam 
     :   forall x T t12 v2 
     ,   value v2 
-    ->  STEP  (XApp (XLam x T t12) v2)
-              (subst x v2 t12)
+    ->  STEP (XApp (XLam x T t12) v2)
+             (substXX x v2 t12)
 
   | EVApp1 
     :   forall t1 t1' t2
@@ -16,7 +16,18 @@ Inductive STEP : exp -> exp -> Prop :=
   | EVApp2
     :   forall v1 t2 t2'
     ,   value v1
-    ->  STEP  t2 t2'
-    ->  STEP  (XApp v1 t2) (XApp v1 t2').
+    ->  STEP t2 t2'
+    ->  STEP (XApp v1 t2) (XApp v1 t2')
+
+  | EVAPPLAM
+    :   forall x t12 T2 
+    ,   STEP (XAPP (XLAM x t12) T2)
+             (substTX x T2 t12)
+
+  | EVAPP1
+    :   forall t1 T2 t1'
+    ,   STEP t1 t1'
+    ->  STEP (XAPP t1 T2) (XAPP t1' T2).
+
 
 Hint Constructors STEP.
